zoo_saturn/mpmc_queue_1: Rewrite.

theories/zoo_saturn/mpmc_queue_1.v
@@ -29,9 +29,9 @@ From zoo Require Import
   options.
 
 Implicit Types b : bool.
-Implicit Types l front node back new_back : location.
+Implicit Types front node back new_back : location.
 Implicit Types hist past nodes : list location.
-Implicit Types v t : val.
+Implicit Types v : val.
 Implicit Types vs : list val.
 Implicit Types waiter : gname.
 Implicit Types waiters : gmap gname nat.
@@ -58,147 +58,887 @@ Proof.
   solve_inG.
 Qed.
 
+Module base.
+  Section mpmc_queue_1_G.
+    Context `{mpmc_queue_1_G : MpmcQueue1G Σ}.
+
+    Implicit Types t : location.
+
+    Record mpmc_queue_1_name := {
+      mpmc_queue_1_name_inv : namespace ;
+      mpmc_queue_1_name_history : gname ;
+      mpmc_queue_1_name_front : gname ;
+      mpmc_queue_1_name_model : gname ;
+      mpmc_queue_1_name_waiters : gname ;
+    }.
+    Implicit Type γ : mpmc_queue_1_name.
+
+    #[global] Instance mpmc_queue_1_name_eq_dec : EqDecision mpmc_queue_1_name :=
+      ltac:(solve_decision).
+    #[global] Instance mpmc_queue_1_name_countable :
+      Countable mpmc_queue_1_name.
+    Proof.
+      solve_countable.
+    Qed.
+
+    #[local] Definition history_auth' γ_history hist :=
+      mono_list_auth γ_history (DfracOwn 1) hist.
+    #[local] Definition history_auth γ hist :=
+      history_auth' γ.(mpmc_queue_1_name_history) hist.
+    #[local] Definition history_at γ i node :=
+      mono_list_at γ.(mpmc_queue_1_name_history) i node.
+
+    #[local] Definition front_auth' γ_front i :=
+      auth_nat_max_auth γ_front (DfracOwn 1) i.
+    #[local] Definition front_auth γ i :=
+      front_auth' γ.(mpmc_queue_1_name_front) i.
+    #[local] Definition front_lb γ i :=
+      auth_nat_max_lb γ.(mpmc_queue_1_name_front) i.
+
+    #[local] Definition model₁' γ_model vs :=
+      twins_twin1 γ_model (DfracOwn 1) vs.
+    #[local] Definition model₁ γ vs :=
+      model₁' γ.(mpmc_queue_1_name_model) vs.
+    #[local] Definition model₂' γ_model vs :=
+      twins_twin2 γ_model vs.
+    #[local] Definition model₂ γ vs :=
+      model₂' γ.(mpmc_queue_1_name_model) vs.
+
+    #[local] Definition waiters_auth' γ_waiters waiters :=
+      ghost_map_auth γ_waiters 1 waiters.
+    #[local] Definition waiters_auth γ waiters :=
+      waiters_auth' γ.(mpmc_queue_1_name_waiters) waiters.
+    #[local] Definition waiters_at γ waiter i :=
+      ghost_map_elem γ.(mpmc_queue_1_name_waiters) waiter (DfracOwn 1) i.
+
+    #[local] Definition node_model γ node i b : iProp Σ :=
+      node ↦ₕ Header §Node 2 ∗
+      history_at γ i node ∗
+      if b then front_lb γ i else True%I.
+    #[local] Instance : CustomIpatFormat "node_model" :=
+      " ( #H{}_header &
+          #Hhistory_at_{} &
+          {{front}#Hfront_lb_{};_}
+        )
+      ".
+
+    #[local] Definition waiter_au γ (Ψ : bool → iProp Σ) : iProp Σ :=
+      AU <{
+        ∃∃ vs,
+        model₁ γ vs
+      }> @ ⊤ ∖ ↑γ.(mpmc_queue_1_name_inv), ∅ <{
+        model₁ γ vs
+      , COMM
+        Ψ (bool_decide (vs = []))
+      }>.
+    #[local] Definition waiter_model γ past waiter i : iProp Σ :=
+      ∃ Ψ,
+      saved_pred waiter Ψ ∗
+      if decide (i < length past) then
+        Ψ false
+      else
+        waiter_au γ Ψ.
+
+    #[local] Definition inv_inner t γ : iProp Σ :=
+      ∃ hist past front nodes back vs waiters,
+      ⌜hist = past ++ front :: nodes⌝ ∗
+      ⌜back ∈ hist⌝ ∗
+      t.[front] ↦ #front ∗
+      t.[back] ↦ #back ∗
+      xtchain (Header §Node 2) (DfracOwn 1) hist §Null ∗
+      ([∗ list] node; v ∈ nodes; vs, node.[data] ↦ v) ∗
+      history_auth γ hist ∗
+      front_auth γ (length past) ∗
+      model₂ γ vs ∗
+      waiters_auth γ waiters ∗
+      ([∗ map] waiter ↦ i ∈ waiters, waiter_model γ past waiter i).
+    #[local] Instance : CustomIpatFormat "inv_inner" :=
+      " ( %hist{} &
+          %past{} &
+          %front{} &
+          %nodes{} &
+          %back{} &
+          %vs{} &
+          %waiters{} &
+          >%Hhist{} &
+          >%Hback{} &
+          >Ht_front &
+          >Ht_back &
+          >Hhist &
+          >Hnodes &
+          >Hhistory_auth &
+          >Hfront_auth &
+          >Hmodel₂ &
+          >Hwaiters_auth &
+          Hwaiters
+        )
+      ".
+    #[local] Definition inv' t γ :=
+      inv γ.(mpmc_queue_1_name_inv) (inv_inner t γ).
+    Definition mpmc_queue_1_inv t γ ι : iProp Σ :=
+      ⌜ι = γ.(mpmc_queue_1_name_inv)⌝ ∗
+      inv' t γ.
+    #[local] Instance : CustomIpatFormat "inv" :=
+      " ( -> &
+          #Hinv
+        )
+      ".
+
+    Definition mpmc_queue_1_model :=
+      model₁.
+    #[local] Instance : CustomIpatFormat "model" :=
+      " Hmodel₁{_{}}
+      ".
+
+    #[global] Instance mpmc_queue_1_model_timeless γ vs :
+      Timeless (mpmc_queue_1_model γ vs).
+    Proof.
+      apply _.
+    Qed.
+
+    #[global] Instance mpmc_queue_1_inv_persistent t γ ι :
+      Persistent (mpmc_queue_1_inv t γ ι).
+    Proof.
+      apply _.
+    Qed.
+
+    #[local] Lemma history_alloc front :
+      ⊢ |==>
+        ∃ γ_history,
+        history_auth' γ_history [front].
+    Proof.
+      apply mono_list_alloc.
+    Qed.
+    #[local] Lemma history_at_get {γ hist} i node :
+      hist !! i = Some node →
+      history_auth γ hist ⊢
+      history_at γ i node.
+    Proof.
+      apply mono_list_at_get.
+    Qed.
+    #[local] Lemma history_at_lookup γ hist i node :
+      history_auth γ hist -∗
+      history_at γ i node -∗
+      ⌜hist !! i = Some node⌝.
+    Proof.
+      apply mono_list_at_valid.
+    Qed.
+    #[local] Lemma history_update {γ hist} node :
+      history_auth γ hist ⊢ |==>
+        history_auth γ (hist ++ [node]) ∗
+        history_at γ (length hist) node.
+    Proof.
+      iIntros "Hauth".
+      iMod (mono_list_update_snoc with "Hauth") as "Hauth".
+      iDestruct (history_at_get with "Hauth") as "#Hat".
+      { rewrite lookup_snoc_Some. naive_solver. }
+      iSteps.
+    Qed.
+
+    #[local] Lemma front_alloc :
+      ⊢ |==>
+        ∃ γ_front,
+        front_auth' γ_front 0.
+    Proof.
+      apply auth_nat_max_alloc.
+    Qed.
+    #[local] Lemma front_lb_get γ i :
+      front_auth γ i ⊢
+      front_lb γ i.
+    Proof.
+      apply auth_nat_max_lb_get.
+    Qed.
+    #[local] Lemma front_lb_valid γ i1 i2 :
+      front_auth γ i1 -∗
+      front_lb γ i2 -∗
+      ⌜i2 ≤ i1⌝.
+    Proof.
+      apply auth_nat_max_lb_valid.
+    Qed.
+    #[local] Lemma front_update {γ i} i' :
+      i ≤ i' →
+      front_auth γ i ⊢ |==>
+      front_auth γ i'.
+    Proof.
+      apply auth_nat_max_update.
+    Qed.
+
+    #[local] Lemma model_alloc :
+      ⊢ |==>
+        ∃ γ_model,
+        model₁' γ_model [] ∗
+        model₂' γ_model [].
+    Proof.
+      apply twins_alloc'.
+    Qed.
+    #[local] Lemma model₁_exclusive γ vs1 vs2 :
+      model₁ γ vs1 -∗
+      model₁ γ vs2 -∗
+      False.
+    Proof.
+      apply twins_twin1_exclusive.
+    Qed.
+    #[local] Lemma model_agree γ vs1 vs2 :
+      model₁ γ vs1 -∗
+      model₂ γ vs2 -∗
+      ⌜vs1 = vs2⌝.
+    Proof.
+      apply: twins_agree_L.
+    Qed.
+    #[local] Lemma model_update {γ vs1 vs2} vs :
+      model₁ γ vs1 -∗
+      model₂ γ vs2 ==∗
+        model₁ γ vs ∗
+        model₂ γ vs.
+    Proof.
+      apply twins_update.
+    Qed.
+
+    #[local] Lemma waiters_alloc :
+      ⊢ |==>
+        ∃ γ_waiters,
+        waiters_auth' γ_waiters ∅.
+    Proof.
+      iMod ghost_map_alloc as "(%γ_waiters & Hwaiters_auth & _)".
+      iSteps.
+    Qed.
+    #[local] Lemma waiters_insert {γ waiters} i Ψ :
+      waiters_auth γ waiters ⊢ |==>
+        ∃ waiter,
+        waiters_auth γ (<[waiter := i]> waiters) ∗
+        saved_pred waiter Ψ ∗
+        waiters_at γ waiter i.
+    Proof.
+      iIntros "Hwaiters_auth".
+      iMod (saved_pred_alloc_cofinite (dom waiters) Ψ) as "(%waiter & %Hwaiter & $)".
+      rewrite not_elem_of_dom in Hwaiter.
+      iApply (ghost_map_insert with "Hwaiters_auth"); first done.
+    Qed.
+    #[local] Lemma waiters_delete γ waiters waiter i :
+      waiters_auth γ waiters -∗
+      waiters_at γ waiter i ==∗
+        ⌜waiters !! waiter = Some i⌝ ∗
+        waiters_auth γ (delete waiter waiters).
+    Proof.
+      iIntros "Hwaiters_auth Hwaiters_at".
+      iDestruct (ghost_map_lookup with "Hwaiters_auth Hwaiters_at") as %?.
+      iMod (ghost_map_delete with "Hwaiters_auth Hwaiters_at") as "$".
+      iSteps.
+    Qed.
+
+    Lemma mpmc_queue_1_model_exclusive γ vs1 vs2 :
+      mpmc_queue_1_model γ vs1 -∗
+      mpmc_queue_1_model γ vs2 -∗
+      False.
+    Proof.
+      iIntros "(:model =1) (:model =2)".
+      iApply (model₁_exclusive with "Hmodel₁_1 Hmodel₁_2").
+    Qed.
+
+    Lemma mpmc_queue_1_create_spec ι :
+      {{{
+        True
+      }}}
+        mpmc_queue_1_create ()
+      {{{ t γ,
+        RET #t;
+        meta_token t ⊤ ∗
+        mpmc_queue_1_inv t γ ι ∗
+        mpmc_queue_1_model γ []
+      }}}.
+    Proof.
+      iIntros "%Φ _ HΦ".
+
+      wp_rec.
+      wp_block front as "#Hfront_header" "_" "(Hfront_next & _)".
+      wp_block t as "Hmeta" "(Ht_front & Ht_back & _)".
+
+      iMod history_alloc as "(%γ_history & Hhistory_auth)".
+      iMod front_alloc as "(%γ_front & Hfront_auth)".
+      iMod model_alloc as "(%γ_model & Hmodel₁ & Hmodel₂)".
+      iMod waiters_alloc as "(%γ_waiters & Hwaiters_auth)".
+
+      pose γ := {|
+        mpmc_queue_1_name_inv := ι ;
+        mpmc_queue_1_name_history := γ_history ;
+        mpmc_queue_1_name_front := γ_front ;
+        mpmc_queue_1_name_model := γ_model ;
+        mpmc_queue_1_name_waiters := γ_waiters ;
+      |}.
+
+      iApply ("HΦ" $! t γ).
+      iFrameStep.
+      iApply inv_alloc.
+      iExists [front], [], front, [], front, [], ∅. iFrameSteps.
+      - rewrite list_elem_of_singleton //.
+      - rewrite xtchain_singleton big_sepM_empty. iSteps.
+    Qed.
+
+    #[local] Lemma front_spec_strong Ψ t γ :
+      {{{
+        inv' t γ ∗
+        if Ψ is Some Ψ then
+          waiter_au γ Ψ
+        else
+          True
+      }}}
+        (#t).{front}
+      {{{ front i,
+        RET #front;
+        node_model γ front i true ∗
+        if Ψ is Some Ψ then
+          ∃ waiter,
+          saved_pred waiter Ψ ∗
+          waiters_at γ waiter i
+        else
+          True
+      }}}.
+    Proof.
+      iIntros "%Φ (#Hinv & HΨ) HΦ".
+
+      iInv "Hinv" as "(:inv_inner)".
+      wp_load.
+      assert (hist !! (length past) = Some front) as Hlookup.
+      { rewrite Hhist list_lookup_middle //. }
+      iDestruct (xtchain_lookup_header with "Hhist") as "#Hfront_header"; first done.
+      iDestruct (history_at_get _ front with "Hhistory_auth") as "#Hhistory_at_front"; first done.
+      iDestruct (front_lb_get with "Hfront_auth") as "#Hfront_lb_front".
+      destruct Ψ as [Ψ |]; last iSteps.
+      iMod (waiters_insert (length past) Ψ with "Hwaiters_auth") as "(%waiter & Hwaiter_auth & #Hwaiter & Hwaiters_at)".
+      iDestruct (big_sepM_insert_2 _ _ waiter (length past) with "[HΨ] Hwaiters") as "Hwaiters".
+      { iExists Ψ. rewrite decide_False; first lia. iSteps. }
+      iSplitR "Hwaiters_at HΦ". { iFrameSteps. }
+      iSteps.
+    Qed.
+    #[local] Lemma front_spec t γ :
+      {{{
+        inv' t γ
+      }}}
+        (#t).{front}
+      {{{ front i,
+        RET #front;
+        node_model γ front i true
+      }}}.
+    Proof.
+      iIntros "%Φ #Hinv HΦ".
+      wp_apply (front_spec_strong None with "[$Hinv]").
+      iSteps.
+    Qed.
+
+    #[local] Lemma back_spec t γ :
+      {{{
+        inv' t γ
+      }}}
+        (#t).{back}
+      {{{ back i,
+        RET #back;
+        node_model γ back i false
+      }}}.
+    Proof.
+      iIntros "%Φ #Hinv HΦ".
+
+      iInv "Hinv" as "(:inv_inner)".
+      wp_load.
+      pose proof Hback as (i & Hlookup)%list_elem_of_lookup.
+      iDestruct (xtchain_lookup_header with "Hhist") as "#Hback_header"; first done.
+      iDestruct (history_at_get with "Hhistory_auth") as "#Hhistory_at_back"; first done.
+      iSplitR "HΦ". { iFrameSteps. }
+      iSteps.
+    Qed.
+
+    Inductive operation :=
+      | IsEmpty waiter (Ψ : bool → iProp Σ)
+      | Pop (Ψ : option val → iProp Σ)
+      | Other.
+    Implicit Types op : operation.
+    Inductive operation' :=
+      | IsEmpty'
+      | Pop'
+      | Other'.
+    #[local] Instance operation'_eq_dec : EqDecision operation' :=
+      ltac:(solve_decision).
+    #[local] Coercion operation_to_operation' op :=
+      match op with
+      | IsEmpty _ _ =>
+          IsEmpty'
+      | Pop _ =>
+          Pop'
+      | Other =>
+          Other'
+      end.
+    #[local] Definition pop_au γ (Ψ : option val → iProp Σ) : iProp Σ :=
+      AU <{
+        ∃∃ vs,
+        model₁ γ vs
+      }> @ ⊤ ∖ ↑γ.(mpmc_queue_1_name_inv), ∅ <{
+        model₁ γ (tail vs)
+      , COMM
+        Ψ (head vs)
+      }>.
+    #[local] Lemma next_spec_aux op t γ i node :
+      {{{
+        inv' t γ ∗
+        history_at γ i node ∗
+        ( if decide (op = Other' :> operation') then True else
+            front_lb γ i
+        ) ∗
+        match op with
+        | IsEmpty waiter Ψ =>
+            saved_pred waiter Ψ ∗
+            waiters_at γ waiter i ∗
+            £ 1
+        | Pop Ψ =>
+            pop_au γ Ψ
+        | Other =>
+            True
+        end
+      }}}
+        (#node).{next}
+      {{{ res,
+        RET res;
+          ⌜res = §Null%V⌝ ∗
+          match op with
+          | IsEmpty waiter Ψ =>
+              Ψ true
+          | Pop Ψ =>
+              Ψ None
+          | Other =>
+              True
+          end
+        ∨ ∃ node',
+          ⌜res = #node'⌝ ∗
+          node_model γ node' (S i) false ∗
+          match op with
+          | IsEmpty waiter Ψ =>
+              Ψ false
+          | Pop Ψ =>
+              pop_au γ Ψ
+          | Other =>
+              True
+          end
+      }}}.
+    Proof.
+      iIntros "%Φ (#Hinv & #Hhistory_at_node & Hop) HΦ".
+
+      iInv "Hinv" as "(:inv_inner)".
+      iDestruct (history_at_lookup with "Hhistory_auth Hhistory_at_node") as %Hlookup.
+      iDestruct (xtchain_lookup_acc with "Hhist") as "(_ & Hnode & Hhist)"; first done.
+      wp_load.
+      iDestruct ("Hhist" with "Hnode") as "Hhist".
+      destruct (hist !! S i) as [node' |] eqn:Hlookup'; simpl.
+
+      - iDestruct (xtchain_lookup_header with "Hhist") as "#Hnode'_header"; first done.
+        iDestruct (history_at_get (S i) with "Hhistory_auth") as "#Hhistory_at_node'"; first done.
+        destruct op; [| iSteps..].
+        iDestruct "Hop" as "(#Hfront_lb_node & #Hwaiter & Hwaiters_at & H£)".
+        iMod (waiters_delete with "Hwaiters_auth Hwaiters_at") as "(%Hwaiters_lookup & Hwaiters_auth)".
+        iDestruct (big_sepM_delete with "Hwaiters") as "((%Ψ_ & Hwaiter_ & HΨ) & Hwaiters)"; first done.
+        iDestruct (saved_pred_agree false with "Hwaiter Hwaiter_") as "Heq".
+        iMod (lc_fupd_elim_later with "H£ Heq") as "Heq".
+        destruct_decide (i = length past) as -> | Hi.
+
+        + rewrite decide_False; first lia.
+
+          iMod "HΨ" as "(%vs_ & Hmodel₁ & _ & HΨ)".
+          iDestruct (model_agree with "Hmodel₁ Hmodel₂") as %->.
+          iMod ("HΨ" with "Hmodel₁") as "HΨ".
+          assert (nodes ≠ []) as Hnodes.
+          { apply lookup_lt_Some in Hlookup'.
+            rewrite Hhist length_app /= in Hlookup'.
+            naive_solver lia.
+          }
+          iAssert ⌜vs ≠ []⌝%I as %Hvs.
+          { destruct_decide (vs = []) as -> | ?; last done.
+            iDestruct (big_sepL2_length with "Hnodes") as %->%nil_length_inv.
+            iSteps.
+          }
+          rewrite bool_decide_eq_false_2 //.
+
+          iSplitR "Heq HΨ HΦ". { iFrameSteps. }
+          iSteps. iRewrite "Heq". iSteps.
+
+        + iDestruct (front_lb_valid with "Hfront_auth Hfront_lb_node") as %Hi_.
+          rewrite decide_True; first lia.
+          iSplitR "Heq HΨ HΦ". { iFrameSteps. }
+          iSteps. iRewrite "Heq". iSteps.
+
+      - destruct_decide (op = Other' :> operation').
+        { destruct op; try done. iSteps. }
+        iDestruct "Hop" as "(#Hfront_lb_node & Hop)".
+        iDestruct (front_lb_valid with "Hfront_auth Hfront_lb_node") as %Hi.
+        opose proof* length_lookup_last as Hlength; [done.. |].
+        rewrite Hhist length_app /= in Hlength.
+        assert (i = length past) as -> by lia.
+        assert (length nodes = 0) as ->%nil_length_inv by lia.
+        iDestruct (big_sepL2_length with "Hnodes") as %->%symmetry%nil_length_inv.
+        destruct op; last done.
+
+        + iDestruct "Hop" as "(#Hwaiter & Hwaiters_at & H£)".
+          iMod (waiters_delete with "Hwaiters_auth Hwaiters_at") as "(%Hwaiters_lookup & Hwaiters_auth)".
+          iDestruct (big_sepM_delete with "Hwaiters") as "((%Ψ_ & Hwaiter_ & HΨ) & Hwaiters)"; first done.
+          iDestruct (saved_pred_agree true with "Hwaiter Hwaiter_") as "Heq".
+          iMod (lc_fupd_elim_later with "H£ Heq") as "Heq".
+          rewrite decide_False; first lia.
+
+          iMod "HΨ" as "(%vs & Hmodel₁ & _ & HΨ)".
+          iDestruct (model_agree with "Hmodel₁ Hmodel₂") as %->.
+          iMod ("HΨ" with "Hmodel₁") as "HΨ".
+
+          iSplitR "Heq HΨ HΦ". { iFrameSteps. }
+          iIntros "!> {%}".
+
+          iApply "HΦ".
+          iLeft. iRewrite "Heq". iSteps.
+
+        + iMod "Hop" as "(%vs & Hmodel₁ & _ & HΨ)".
+          iDestruct (model_agree with "Hmodel₁ Hmodel₂") as %->.
+          iMod ("HΨ" with "Hmodel₁") as "HΨ".
+
+          iSplitR "HΨ HΦ". { iFrameSteps. }
+          iSteps.
+    Qed.
+    #[local] Lemma next_spec {t γ i} node :
+      {{{
+        inv' t γ ∗
+        history_at γ i node
+      }}}
+        (#node).{next}
+      {{{ res,
+        RET res;
+          ⌜res = §Null%V⌝
+        ∨ ∃ node',
+          ⌜res = #node'⌝ ∗
+          node_model γ node' (S i) false
+      }}}.
+    Proof.
+      iIntros "%Φ (#Hinv & #Hhistory_at_node) HΦ".
+      wp_apply (next_spec_aux Other); iSteps.
+    Qed.
+    #[local] Lemma next_spec_is_empty {t γ i node} waiter Ψ :
+      {{{
+        inv' t γ ∗
+        history_at γ i node ∗
+        front_lb γ i ∗
+        saved_pred waiter Ψ ∗
+        waiters_at γ waiter i ∗
+        £ 1
+      }}}
+        (#node).{next}
+      {{{ res,
+        RET res;
+          ⌜res = §Null%V⌝ ∗
+          Ψ true
+        ∨ ∃ node',
+          ⌜res = #node'⌝ ∗
+          node_model γ node' (S i) false ∗
+          Ψ false
+      }}}.
+    Proof.
+      iIntros "%Φ (#Hinv & #Hhistory_at_node & #Hfront_lb_node & #Hwaiter & Hwaiters_at & H£) HΦ".
+      wp_apply (next_spec_aux (IsEmpty _ _) with "[$]").
+      iSteps.
+    Qed.
+    #[local] Lemma next_spec_pop {t γ i node} Ψ :
+      {{{
+        inv' t γ ∗
+        history_at γ i node ∗
+        front_lb γ i ∗
+        pop_au γ Ψ
+      }}}
+        (#node).{next}
+      {{{ res,
+        RET res;
+          ⌜res = §Null%V⌝ ∗
+          Ψ None
+        ∨ ∃ node',
+          ⌜res = #node'⌝ ∗
+          node_model γ node' (S i) false ∗
+          pop_au γ Ψ
+      }}}.
+    Proof.
+      iIntros "%Φ (#Hinv & #Hhistory_at_node & #Hfront_lb_node & Hau) HΦ".
+      wp_apply (next_spec_aux (Pop _) with "[$]").
+      iSteps.
+    Qed.
+
+    Lemma mpmc_queue_1_is_empty_spec t γ ι :
+      <<<
+        mpmc_queue_1_inv t γ ι
+      | ∀∀ vs,
+        mpmc_queue_1_model γ vs
+      >>>
+        mpmc_queue_1_is_empty #t @ ↑ι
+      <<<
+        mpmc_queue_1_model γ vs
+      | RET #(bool_decide (vs = []%list));
+        £ 1
+      >>>.
+    Proof.
+      iIntros "%Φ (:inv) HΦ".
+
+      wp_rec credits:"H£".
+      iDestruct (lc_weaken 2 with "H£") as "(H£1 & H£2)"; first done.
+      iDestruct (atomic_update_frame_l with "[H£1 $HΦ]") as "HΦ"; first iAccu.
+
+      wp_smart_apply (front_spec_strong (Some $ λ b, Φ #b) with "[$Hinv HΦ]")
+      as (node i) "((:node_model =node front=) & %waiter & #Hwaiter & Hwaiters_at)".
+      { rewrite /= /waiter_au. iAuIntro.
+        iApply (aacc_aupd_commit with "HΦ"); first done. iIntros "%vs (:model)".
+        iAaccIntro with "Hmodel₁"; iSteps.
+      }
+      wp_match.
+      wp_smart_apply (next_spec_is_empty with "[$]"); iSteps.
+    Qed.
+    Lemma mpmc_queue_1_is_empty_spec' t γ ι :
+      {{{
+        mpmc_queue_1_inv t γ ι
+      }}}
+        mpmc_queue_1_is_empty #t
+      {{{ b,
+        RET #b;
+        True
+      }}}.
+    Proof.
+      iIntros "%Φ (:inv) HΦ".
+
+      wp_rec.
+      wp_apply (front_spec with "Hinv") as (front i) "(:node_model =front front=)".
+      wp_match.
+      wp_apply (next_spec with "[$]") as (res) "[-> | (%node & -> & _)]"; iSteps.
+    Qed.
+
+    #[local] Lemma mpmc_queue_1_push_0_spec t γ i node new_back v :
+      <<<
+        inv' t γ ∗
+        node_model γ node i false ∗
+        new_back ↦ₕ Header §Node 2 ∗
+        new_back.[next] ↦ §Null ∗
+        new_back.[data] ↦ v
+      | ∀∀ vs,
+        mpmc_queue_1_model γ vs
+      >>>
+        mpmc_queue_1_push_0 #node #new_back @ ↑γ.(mpmc_queue_1_name_inv)
+      <<<
+        mpmc_queue_1_model γ (vs ++ [v])
+      | RET ();
+        ∃ j,
+        history_at γ j new_back
+      >>>.
+    Proof.
+      iIntros "%Φ (#Hinv & (:node_model =node) & #Hnew_back_header & Hnew_back_next & Hnew_back_data) HΦ".
+
+      iLöb as "HLöb" forall (i node) "Hnode_header Hhistory_at_node".
+
+      wp_rec. wp_match.
+      wp_smart_apply (next_spec with "[$]") as (res) "[-> | (%node' & -> & (:node_model =node'))]"; last iSteps.
+      wp_pures.
+
+      wp_bind (CAS _ _ _).
+      iInv "Hinv" as "(:inv_inner)".
+      iDestruct (history_at_lookup with "Hhistory_auth Hhistory_at_node") as %Hlookup.
+      iDestruct (xtchain_lookup with "Hhist") as "(Hhist1 & _ & Hnode & Hhist2)"; first done.
+      destruct (hist !! S i) as [node' |] eqn:Hlookup'; simpl.
+
+      - wp_cas as _ | [=].
+        iDestruct (xtchain_lookup_2 with "Hhist1 Hnode_header Hnode Hhist2") as "Hhist"; [done | rewrite Hlookup' // |].
+        iSplitR "Hnew_back_next Hnew_back_data HΦ". { iFrameSteps. }
+        iSteps.
+
+      - wp_cas as ? | _; first done.
+        iDestruct (xtchain_lookup_2 with "Hhist1 Hnode_header Hnode []") as "Hhist"; [done | rewrite Hlookup' // | ..].
+        { rewrite -(length_lookup_last hist i) // drop_all.
+          iApply xtchain_nil.
+        }
+        iDestruct (big_sepL2_snoc_2 with "Hnodes Hnew_back_data") as "Hnodes".
+        iDestruct (xtchain_snoc_2 with "Hhist Hnew_back_header Hnew_back_next") as "Hhist".
+        iMod (history_update new_back with "Hhistory_auth") as "(Hhistory_auth & #Hhistory_at_new_back)".
+
+        iMod "HΦ" as "(%vs_ & (:model) & _ & HΦ)".
+        iDestruct (model_agree with "Hmodel₁ Hmodel₂") as %->.
+        iMod (model_update (vs ++ [v]) with "Hmodel₁ Hmodel₂") as "(Hmodel₁ & Hmodel₂)".
+        iMod ("HΦ" with "Hmodel₁") as "HΦ".
+
+        iSplitR "HΦ".
+        { iExists (hist ++ [new_back]), past, front, (nodes ++ [new_back]), back, (vs ++ [v]).
+          iSteps; iPureIntro.
+          - rewrite Hhist -assoc //.
+          - set_solver.
+        }
+        iSteps.
+    Qed.
+
+    #[local] Lemma mpmc_queue_1_fix_back_spec t γ i back j new_back :
+      {{{
+        inv' t γ ∗
+        history_at γ i back ∗
+        node_model γ new_back j false
+      }}}
+        mpmc_queue_1_fix_back #t #back #new_back
+      {{{
+        RET ();
+        True
+      }}}.
+    Proof.
+      iIntros "%Φ (#Hinv & #Hhistory_at_back & (:node_model =new_back)) HΦ".
+
+      iLöb as "HLöb" forall (i back) "Hhistory_at_back".
+
+      wp_rec. wp_match.
+
+      wp_bind (_ and _)%E.
+      wp_apply (wp_wand itype_bool) as (res) "(%b & ->)".
+      { wp_smart_apply (next_spec new_back with "[$]") as (res) "[-> | (%new_back' & -> & (:node_model =new_back'))]"; last iSteps.
+        wp_pures.
+
+        wp_bind (CAS _ _ _).
+        iInv "Hinv" as "(:inv_inner =1)".
+        wp_cas as _ | [= ->]; first iSteps.
+        iDestruct (history_at_lookup with "Hhistory_auth Hhistory_at_new_back") as %Hnew_back%list_elem_of_lookup_2.
+        iSteps.
+      }
+
+      destruct b; last iSteps.
+      wp_smart_apply domain_yield_spec.
+      wp_smart_apply (back_spec with "Hinv") as (back' i') "(:node_model =back')".
+      iApply ("HLöb" with "HΦ Hhistory_at_back'").
+    Qed.
+
+    Lemma mpmc_queue_1_push_spec t γ ι v :
+      <<<
+        mpmc_queue_1_inv t γ ι
+      | ∀∀ vs,
+        mpmc_queue_1_model γ vs
+      >>>
+        mpmc_queue_1_push #t v @ ↑ι
+      <<<
+        mpmc_queue_1_model γ (vs ++ [v])
+      | RET ();
+        £ 1
+      >>>.
+    Proof.
+      iIntros "%Φ (:inv) HΦ".
+
+      wp_rec credit:"H£".
+      iDestruct (atomic_update_frame_l with "[H£ $HΦ]") as "HΦ"; first iAccu.
+      wp_block new_back as "#Hnew_back_header" "_" "(Hnew_back_next & Hnew_back_data & _)".
+      wp_match.
+      wp_smart_apply (back_spec with "Hinv") as (back i) "(:node_model =back)".
+      wp_smart_apply (mpmc_queue_1_push_0_spec with "[$]").
+      iApply (atomic_update_wand with "HΦ"). iIntros "%vs HΦ (%j & #Hhistory_at_new_back)".
+      wp_smart_apply (mpmc_queue_1_fix_back_spec with "[]"); first iSteps.
+      iSteps.
+    Qed.
+
+    Lemma mpmc_queue_1_pop_spec t γ ι :
+      <<<
+        mpmc_queue_1_inv t γ ι
+      | ∀∀ vs,
+        mpmc_queue_1_model γ vs
+      >>>
+        mpmc_queue_1_pop #t @ ↑ι
+      <<<
+        mpmc_queue_1_model γ (tail vs)
+      | RET head vs;
+        £ 1
+      >>>.
+    Proof.
+      iIntros "%Φ (:inv) HΦ".
+
+      iLöb as "HLöb".
+
+      wp_rec credit:"H£".
+      wp_smart_apply (front_spec with "Hinv") as (front i) "(:node_model =front front=)".
+      wp_match.
+      wp_smart_apply (next_spec_pop (λ o, _ -∗ Φ o)%I with "[$]") as (res) "[(-> & HΦ) | (%new_front & -> & (:node_model =new_front) & HΦ)]"; first iSteps.
+      wp_match. wp_pures.
+
+      wp_bind (CAS _ _ _).
+      iInv "Hinv" as "(:inv_inner =1)".
+      iDestruct (history_at_lookup with "Hhistory_auth Hhistory_at_new_front") as %Hlookup.
+      iDestruct (xtchain_lookup_acc with "Hhist") as "(_ & Hnode & Hhist)"; first done.
+      wp_cas as _ | [= <-]; first iSteps.
+      iDestruct ("Hhist" with "Hnode") as "Hhist".
+      iDestruct (history_at_lookup with "Hhistory_auth Hhistory_at_front") as %Hlookup_old.
+      iAssert ⌜length past1 = i⌝%I as %Hpast_length.
+      { iDestruct (xtchain_NoDup with "Hhist") as %Hnodup.
+        iPureIntro. eapply NoDup_lookup; try done.
+        rewrite Hhist1 list_lookup_middle //.
+      }
+      rewrite Hhist1 (assoc _ _ [_]) lookup_app_r length_app /= in Hlookup; first lia.
+      rewrite Nat.add_1_r Hpast_length Nat.sub_diag in Hlookup.
+      destruct nodes1 as [| node nodes1]; first done. injection Hlookup as ->.
+      rewrite (assoc _ _ [_]) in Hhist1.
+      iDestruct (big_sepL2_cons_inv_l with "Hnodes") as "(%v & %vs' & -> & Hfront_data & Hnodes)".
+      set past := past1 ++ [front].
+      iMod (front_update (length past) with "Hfront_auth") as "Hfront_auth".
+      { rewrite /past. simpl_length. lia. }
+      iDestruct (big_sepM_impl_thread_fupd _ (waiter_model γ past)%I with "Hwaiters Hmodel₂ [#]") as ">(Hwaiters & Hmodel₂)".
+      { iIntros "!> %waiter %j %Hlookup (%P & #Hwaiter & HP) Hmodel₂".
+        destruct (Nat.lt_trichotomy j (length past1)) as [Hj | [-> | Hj]].
+        - rewrite decide_True //.
+          rewrite /waiter_model. setoid_rewrite decide_True; last first.
+          { rewrite /past. simpl_length. lia. }
+          iSteps.
+        - rewrite decide_False; first lia.
+          rewrite /waiter_model. setoid_rewrite decide_True; last first.
+          { rewrite /past. simpl_length/=. lia. }
+          iMod "HP" as "(%vs & Hmodel₁ & _ & HP)".
+          iDestruct (model_agree with "Hmodel₁ Hmodel₂") as %->.
+          iSteps.
+        - rewrite decide_False; first lia.
+          rewrite /waiter_model. setoid_rewrite decide_False; last first.
+          { rewrite /past. simpl_length/=. lia. }
+          iSteps.
+      }
+
+      iMod "HΦ" as "(%vs & Hmodel₁ & _ & HΦ)".
+      iDestruct (model_agree with "Hmodel₁ Hmodel₂") as %->.
+      iMod (model_update vs' with "Hmodel₁ Hmodel₂") as "(Hmodel₁ & Hmodel₂)".
+      iMod ("HΦ" with "Hmodel₁") as "HΦ".
+
+      iSplitR "Hfront_data H£ HΦ". { iFrameSteps. }
+      iSteps.
+    Qed.
+  End mpmc_queue_1_G.
+
+  #[global] Opaque mpmc_queue_1_inv.
+  #[global] Opaque mpmc_queue_1_model.
+End base.
+
+From zoo_saturn Require
+  mpmc_queue_1__opaque.
+
 Section mpmc_queue_1_G.
   Context `{mpmc_queue_1_G : MpmcQueue1G Σ}.
 
-  Record metadata := {
-    metadata_inv : namespace ;
-    metadata_history : gname ;
-    metadata_front : gname ;
-    metadata_model : gname ;
-    metadata_waiters : gname ;
-  }.
-  Implicit Type γ : metadata.
+  Implicit Types 𝑡 : location.
+  Implicit Types t : val.
 
-  #[local] Instance metadata_eq_dec : EqDecision metadata :=
-    ltac:(solve_decision).
-  #[local] Instance metadata_countable :
-    Countable metadata.
-  Proof.
-    solve_countable.
-  Qed.
-
-  #[local] Definition history_auth' γ_history hist :=
-    mono_list_auth γ_history (DfracOwn 1) hist.
-  #[local] Definition history_auth γ hist :=
-    history_auth' γ.(metadata_history) hist.
-  #[local] Definition history_at γ i node :=
-    mono_list_at γ.(metadata_history) i node.
-
-  #[local] Definition front_auth' γ_front i :=
-    auth_nat_max_auth γ_front (DfracOwn 1) i.
-  #[local] Definition front_auth γ i :=
-    front_auth' γ.(metadata_front) i.
-  #[local] Definition front_lb γ i :=
-    auth_nat_max_lb γ.(metadata_front) i.
-
-  #[local] Definition model₁' γ_model vs :=
-    twins_twin1 γ_model (DfracOwn 1) vs.
-  #[local] Definition model₁ γ vs :=
-    model₁' γ.(metadata_model) vs.
-  #[local] Definition model₂' γ_model vs :=
-    twins_twin2 γ_model vs.
-  #[local] Definition model₂ γ vs :=
-    model₂' γ.(metadata_model) vs.
-
-  #[local] Definition waiters_auth' γ_waiters waiters :=
-    ghost_map_auth γ_waiters 1 waiters.
-  #[local] Definition waiters_auth γ waiters :=
-    waiters_auth' γ.(metadata_waiters) waiters.
-  #[local] Definition waiters_at γ waiter i :=
-    ghost_map_elem γ.(metadata_waiters) waiter (DfracOwn 1) i.
-
-  #[local] Definition node_model γ node i b : iProp Σ :=
-    node ↦ₕ Header §Node 2 ∗
-    history_at γ i node ∗
-    if b then front_lb γ i else True%I.
-  #[local] Instance : CustomIpatFormat "node_model" :=
-    " ( #H{}_header &
-        #Hhistory_at_{} &
-        {{front}#Hfront_lb_{};_}
-      )
-    ".
-
-  #[local] Definition waiter_au γ (Ψ : bool → iProp Σ) : iProp Σ :=
-    AU <{
-      ∃∃ vs,
-      model₁ γ vs
-    }> @ ⊤ ∖ ↑γ.(metadata_inv), ∅ <{
-      model₁ γ vs
-    , COMM
-      Ψ (bool_decide (vs = []))
-    }>.
-  #[local] Definition waiter_model γ past waiter i : iProp Σ :=
-    ∃ Ψ,
-    saved_pred waiter Ψ ∗
-    if decide (i < length past) then
-      Ψ false
-    else
-      waiter_au γ Ψ.
-
-  #[local] Definition inv_inner l γ : iProp Σ :=
-    ∃ hist past front nodes back vs waiters,
-    ⌜hist = past ++ front :: nodes⌝ ∗
-    ⌜back ∈ hist⌝ ∗
-    l.[front] ↦ #front ∗
-    l.[back] ↦ #back ∗
-    xtchain (Header §Node 2) (DfracOwn 1) hist §Null ∗
-    ([∗ list] node; v ∈ nodes; vs, node.[data] ↦ v) ∗
-    history_auth γ hist ∗
-    front_auth γ (length past) ∗
-    model₂ γ vs ∗
-    waiters_auth γ waiters ∗
-    ([∗ map] waiter ↦ i ∈ waiters, waiter_model γ past waiter i).
-  #[local] Instance : CustomIpatFormat "inv_inner" :=
-    " ( %hist{} &
-        %past{} &
-        %front{} &
-        %nodes{} &
-        %back{} &
-        %vs{} &
-        %waiters{} &
-        >%Hhist{} &
-        >%Hback{} &
-        >Hl_front &
-        >Hl_back &
-        >Hhist &
-        >Hnodes &
-        >Hhistory_auth &
-        >Hfront_auth &
-        >Hmodel₂ &
-        >Hwaiters_auth &
-        Hwaiters
-      )
-    ".
-  #[local] Definition inv' l γ :=
-    inv γ.(metadata_inv) (inv_inner l γ).
   Definition mpmc_queue_1_inv t ι : iProp Σ :=
-    ∃ l γ,
-    ⌜t = #l⌝ ∗
-    ⌜ι = γ.(metadata_inv)⌝ ∗
-    meta l nroot γ ∗
-    inv' l γ.
+    ∃ 𝑡 γ,
+    ⌜t = #𝑡⌝ ∗
+    meta 𝑡 nroot γ ∗
+    base.mpmc_queue_1_inv 𝑡 γ ι.
   #[local] Instance : CustomIpatFormat "inv" :=
-    " ( %l &
-        %γ &
-        -> &
-        -> &
-        #Hmeta &
-        #Hinv
+    " ( %𝑡{} &
+        %γ{} &
+        {%Heq{};->} &
+        #Hmeta{_{}} &
+        Hinv{_{}}
       )
     ".
 
   Definition mpmc_queue_1_model t vs : iProp Σ :=
-    ∃ l γ,
-    ⌜t = #l⌝ ∗
-    meta l nroot γ ∗
-    model₁ γ vs.
+    ∃ 𝑡 γ,
+    ⌜t = #𝑡⌝ ∗
+    meta 𝑡 nroot γ ∗
+    base.mpmc_queue_1_model γ vs.
   #[local] Instance : CustomIpatFormat "model" :=
-    " ( %l{;_} &
-        %γ{;_} &
-        %Heq{} &
-        #Hmeta_{} &
-        Hmodel₁{_{}}
+    " ( %𝑡{} &
+        %γ{} &
+        {%Heq{};->} &
+        Hmeta{_{}} &
+        Hmodel{_{}}
       )
     ".
 
@@ -214,130 +954,6 @@ Section mpmc_queue_1_G.
     apply _.
   Qed.
 
-  #[local] Lemma history_alloc front :
-    ⊢ |==>
-      ∃ γ_history,
-      history_auth' γ_history [front].
-  Proof.
-    apply mono_list_alloc.
-  Qed.
-  #[local] Lemma history_at_get {γ hist} i node :
-    hist !! i = Some node →
-    history_auth γ hist ⊢
-    history_at γ i node.
-  Proof.
-    apply mono_list_at_get.
-  Qed.
-  #[local] Lemma history_at_lookup γ hist i node :
-    history_auth γ hist -∗
-    history_at γ i node -∗
-    ⌜hist !! i = Some node⌝.
-  Proof.
-    apply mono_list_at_valid.
-  Qed.
-  #[local] Lemma history_update {γ hist} node :
-    history_auth γ hist ⊢ |==>
-      history_auth γ (hist ++ [node]) ∗
-      history_at γ (length hist) node.
-  Proof.
-    iIntros "Hauth".
-    iMod (mono_list_update_snoc with "Hauth") as "Hauth".
-    iDestruct (history_at_get with "Hauth") as "#Hat".
-    { rewrite lookup_snoc_Some. naive_solver. }
-    iSteps.
-  Qed.
-
-  #[local] Lemma front_alloc :
-    ⊢ |==>
-      ∃ γ_front,
-      front_auth' γ_front 0.
-  Proof.
-    apply auth_nat_max_alloc.
-  Qed.
-  #[local] Lemma front_lb_get γ i :
-    front_auth γ i ⊢
-    front_lb γ i.
-  Proof.
-    apply auth_nat_max_lb_get.
-  Qed.
-  #[local] Lemma front_lb_valid γ i1 i2 :
-    front_auth γ i1 -∗
-    front_lb γ i2 -∗
-    ⌜i2 ≤ i1⌝.
-  Proof.
-    apply auth_nat_max_lb_valid.
-  Qed.
-  #[local] Lemma front_update {γ i} i' :
-    i ≤ i' →
-    front_auth γ i ⊢ |==>
-    front_auth γ i'.
-  Proof.
-    apply auth_nat_max_update.
-  Qed.
-
-  #[local] Lemma model_alloc :
-    ⊢ |==>
-      ∃ γ_model,
-      model₁' γ_model [] ∗
-      model₂' γ_model [].
-  Proof.
-    apply twins_alloc'.
-  Qed.
-  #[local] Lemma model₁_exclusive γ vs1 vs2 :
-    model₁ γ vs1 -∗
-    model₁ γ vs2 -∗
-    False.
-  Proof.
-    apply twins_twin1_exclusive.
-  Qed.
-  #[local] Lemma model_agree γ vs1 vs2 :
-    model₁ γ vs1 -∗
-    model₂ γ vs2 -∗
-    ⌜vs1 = vs2⌝.
-  Proof.
-    apply: twins_agree_L.
-  Qed.
-  #[local] Lemma model_update {γ vs1 vs2} vs :
-    model₁ γ vs1 -∗
-    model₂ γ vs2 ==∗
-      model₁ γ vs ∗
-      model₂ γ vs.
-  Proof.
-    apply twins_update.
-  Qed.
-
-  #[local] Lemma waiters_alloc :
-    ⊢ |==>
-      ∃ γ_waiters,
-      waiters_auth' γ_waiters ∅.
-  Proof.
-    iMod ghost_map_alloc as "(%γ_waiters & Hwaiters_auth & _)".
-    iSteps.
-  Qed.
-  #[local] Lemma waiters_insert {γ waiters} i Ψ :
-    waiters_auth γ waiters ⊢ |==>
-      ∃ waiter,
-      waiters_auth γ (<[waiter := i]> waiters) ∗
-      saved_pred waiter Ψ ∗
-      waiters_at γ waiter i.
-  Proof.
-    iIntros "Hwaiters_auth".
-    iMod (saved_pred_alloc_cofinite (dom waiters) Ψ) as "(%waiter & %Hwaiter & $)".
-    rewrite not_elem_of_dom in Hwaiter.
-    iApply (ghost_map_insert with "Hwaiters_auth"); first done.
-  Qed.
-  #[local] Lemma waiters_delete γ waiters waiter i :
-    waiters_auth γ waiters -∗
-    waiters_at γ waiter i ==∗
-      ⌜waiters !! waiter = Some i⌝ ∗
-      waiters_auth γ (delete waiter waiters).
-  Proof.
-    iIntros "Hwaiters_auth Hwaiters_at".
-    iDestruct (ghost_map_lookup with "Hwaiters_auth Hwaiters_at") as %?.
-    iMod (ghost_map_delete with "Hwaiters_auth Hwaiters_at") as "$".
-    iSteps.
-  Qed.
-
   Lemma mpmc_queue_1_model_exclusive t vs1 vs2 :
     mpmc_queue_1_model t vs1 -∗
     mpmc_queue_1_model t vs2 -∗
@@ -345,7 +961,7 @@ Section mpmc_queue_1_G.
   Proof.
     iIntros "(:model =1) (:model =2)". simplify.
     iDestruct (meta_agree with "Hmeta_1 Hmeta_2") as %->.
-    iApply (model₁_exclusive with "Hmodel₁_1 Hmodel₁_2").
+    iApply (base.mpmc_queue_1_model_exclusive with "Hmodel_1 Hmodel_2").
   Qed.
 
   Lemma mpmc_queue_1_create_spec ι :
@@ -361,317 +977,9 @@ Section mpmc_queue_1_G.
   Proof.
     iIntros "%Φ _ HΦ".
 
-    wp_rec.
-    wp_block front as "#Hfront_header" "_" "(Hfront_next & _)".
-    wp_block l as "Hmeta" "(Hl_front & Hl_back & _)".
-
-    iMod history_alloc as "(%γ_history & Hhistory_auth)".
-    iMod front_alloc as "(%γ_front & Hfront_auth)".
-    iMod model_alloc as "(%γ_model & Hmodel₁ & Hmodel₂)".
-    iMod waiters_alloc as "(%γ_waiters & Hwaiters_auth)".
-
-    pose γ := {|
-      metadata_inv := ι ;
-      metadata_history := γ_history ;
-      metadata_front := γ_front ;
-      metadata_model := γ_model ;
-      metadata_waiters := γ_waiters ;
-    |}.
-
-    iMod (meta_set γ with "Hmeta") as "#Hmeta"; first done.
-
-    iApply "HΦ".
-    iSplitR "Hmodel₁"; last iSteps.
-    iExists l, γ. iStep 3. iApply inv_alloc.
-    iExists [front], [], front, [], front, [], ∅. iFrameSteps.
-    - rewrite list_elem_of_singleton //.
-    - rewrite xtchain_singleton big_sepM_empty. iSteps.
-  Qed.
-
-  #[local] Lemma front_spec_strong Ψ l γ :
-    {{{
-      inv' l γ ∗
-      if Ψ is Some Ψ then
-        waiter_au γ Ψ
-      else
-        True
-    }}}
-      (#l).{front}
-    {{{ front i,
-      RET #front;
-      node_model γ front i true ∗
-      if Ψ is Some Ψ then
-        ∃ waiter,
-        saved_pred waiter Ψ ∗
-        waiters_at γ waiter i
-      else
-        True
-    }}}.
-  Proof.
-    iIntros "%Φ (#Hinv & HΨ) HΦ".
-
-    iInv "Hinv" as "(:inv_inner)".
-    wp_load.
-    assert (hist !! (length past) = Some front) as Hlookup.
-    { rewrite Hhist list_lookup_middle //. }
-    iDestruct (xtchain_lookup_header with "Hhist") as "#Hfront_header"; first done.
-    iDestruct (history_at_get _ front with "Hhistory_auth") as "#Hhistory_at_front"; first done.
-    iDestruct (front_lb_get with "Hfront_auth") as "#Hfront_lb_front".
-    destruct Ψ as [Ψ |]; last iSteps.
-    iMod (waiters_insert (length past) Ψ with "Hwaiters_auth") as "(%waiter & Hwaiter_auth & #Hwaiter & Hwaiters_at)".
-    iDestruct (big_sepM_insert_2 _ _ waiter (length past) with "[HΨ] Hwaiters") as "Hwaiters".
-    { iExists Ψ. rewrite decide_False; first lia. iSteps. }
-    iSplitR "Hwaiters_at HΦ". { iFrameSteps. }
-    iSteps.
-  Qed.
-  #[local] Lemma front_spec l γ :
-    {{{
-      inv' l γ
-    }}}
-      (#l).{front}
-    {{{ front i,
-      RET #front;
-      node_model γ front i true
-    }}}.
-  Proof.
-    iIntros "%Φ #Hinv HΦ".
-    wp_apply (front_spec_strong None with "[$Hinv]").
-    iSteps.
-  Qed.
-
-  #[local] Lemma back_spec l γ :
-    {{{
-      inv' l γ
-    }}}
-      (#l).{back}
-    {{{ back i,
-      RET #back;
-      node_model γ back i false
-    }}}.
-  Proof.
-    iIntros "%Φ #Hinv HΦ".
-
-    iInv "Hinv" as "(:inv_inner)".
-    wp_load.
-    pose proof Hback as (i & Hlookup)%list_elem_of_lookup.
-    iDestruct (xtchain_lookup_header with "Hhist") as "#Hback_header"; first done.
-    iDestruct (history_at_get with "Hhistory_auth") as "#Hhistory_at_back"; first done.
-    iSplitR "HΦ". { iFrameSteps. }
-    iSteps.
-  Qed.
-
-  Inductive operation :=
-    | IsEmpty waiter (Ψ : bool → iProp Σ)
-    | Pop (Ψ : option val → iProp Σ)
-    | Other.
-  Implicit Types op : operation.
-  Inductive operation' :=
-    | IsEmpty'
-    | Pop'
-    | Other'.
-  #[local] Instance operation'_eq_dec : EqDecision operation' :=
-    ltac:(solve_decision).
-  #[local] Coercion operation_to_operation' op :=
-    match op with
-    | IsEmpty _ _ =>
-        IsEmpty'
-    | Pop _ =>
-        Pop'
-    | Other =>
-        Other'
-    end.
-  #[local] Definition pop_au γ (Ψ : option val → iProp Σ) : iProp Σ :=
-    AU <{
-      ∃∃ vs,
-      model₁ γ vs
-    }> @ ⊤ ∖ ↑γ.(metadata_inv), ∅ <{
-      model₁ γ (tail vs)
-    , COMM
-      Ψ (head vs)
-    }>.
-  #[local] Lemma next_spec_aux op l γ i node :
-    {{{
-      inv' l γ ∗
-      history_at γ i node ∗
-      ( if decide (op = Other' :> operation') then True else
-          front_lb γ i
-      ) ∗
-      match op with
-      | IsEmpty waiter Ψ =>
-          saved_pred waiter Ψ ∗
-          waiters_at γ waiter i ∗
-          £ 1
-      | Pop Ψ =>
-          pop_au γ Ψ
-      | Other =>
-          True
-      end
-    }}}
-      (#node).{next}
-    {{{ res,
-      RET res;
-        ⌜res = §Null%V⌝ ∗
-        match op with
-        | IsEmpty waiter Ψ =>
-            Ψ true
-        | Pop Ψ =>
-            Ψ None
-        | Other =>
-            True
-        end
-      ∨ ∃ node',
-        ⌜res = #node'⌝ ∗
-        node_model γ node' (S i) false ∗
-        match op with
-        | IsEmpty waiter Ψ =>
-            Ψ false
-        | Pop Ψ =>
-            pop_au γ Ψ
-        | Other =>
-            True
-        end
-    }}}.
-  Proof.
-    iIntros "%Φ (#Hinv & #Hhistory_at_node & Hop) HΦ".
-
-    iInv "Hinv" as "(:inv_inner)".
-    iDestruct (history_at_lookup with "Hhistory_auth Hhistory_at_node") as %Hlookup.
-    iDestruct (xtchain_lookup_acc with "Hhist") as "(_ & Hnode & Hhist)"; first done.
-    wp_load.
-    iDestruct ("Hhist" with "Hnode") as "Hhist".
-    destruct (hist !! S i) as [node' |] eqn:Hlookup'; simpl.
-
-    - iDestruct (xtchain_lookup_header with "Hhist") as "#Hnode'_header"; first done.
-      iDestruct (history_at_get (S i) with "Hhistory_auth") as "#Hhistory_at_node'"; first done.
-      destruct op; [| iSteps..].
-      iDestruct "Hop" as "(#Hfront_lb_node & #Hwaiter & Hwaiters_at & H£)".
-      iMod (waiters_delete with "Hwaiters_auth Hwaiters_at") as "(%Hwaiters_lookup & Hwaiters_auth)".
-      iDestruct (big_sepM_delete with "Hwaiters") as "((%Ψ_ & Hwaiter_ & HΨ) & Hwaiters)"; first done.
-      iDestruct (saved_pred_agree false with "Hwaiter Hwaiter_") as "Heq".
-      iMod (lc_fupd_elim_later with "H£ Heq") as "Heq".
-      destruct_decide (i = length past) as -> | Hi.
-
-      + rewrite decide_False; first lia.
-
-        iMod "HΨ" as "(%vs_ & Hmodel₁ & _ & HΨ)".
-        iDestruct (model_agree with "Hmodel₁ Hmodel₂") as %->.
-        iMod ("HΨ" with "Hmodel₁") as "HΨ".
-        assert (nodes ≠ []) as Hnodes.
-        { apply lookup_lt_Some in Hlookup'.
-          rewrite Hhist length_app /= in Hlookup'.
-          naive_solver lia.
-        }
-        iAssert ⌜vs ≠ []⌝%I as %Hvs.
-        { destruct_decide (vs = []) as -> | ?; last done.
-          iDestruct (big_sepL2_length with "Hnodes") as %->%nil_length_inv.
-          iSteps.
-        }
-        rewrite bool_decide_eq_false_2 //.
-
-        iSplitR "Heq HΨ HΦ". { iFrameSteps. }
-        iSteps. iRewrite "Heq". iSteps.
-
-      + iDestruct (front_lb_valid with "Hfront_auth Hfront_lb_node") as %Hi_.
-        rewrite decide_True; first lia.
-        iSplitR "Heq HΨ HΦ". { iFrameSteps. }
-        iSteps. iRewrite "Heq". iSteps.
-
-    - destruct_decide (op = Other' :> operation').
-      { destruct op; try done. iSteps. }
-      iDestruct "Hop" as "(#Hfront_lb_node & Hop)".
-      iDestruct (front_lb_valid with "Hfront_auth Hfront_lb_node") as %Hi.
-      opose proof* length_lookup_last as Hlength; [done.. |].
-      rewrite Hhist length_app /= in Hlength.
-      assert (i = length past) as -> by lia.
-      assert (length nodes = 0) as ->%nil_length_inv by lia.
-      iDestruct (big_sepL2_length with "Hnodes") as %->%symmetry%nil_length_inv.
-      destruct op; last done.
-
-      + iDestruct "Hop" as "(#Hwaiter & Hwaiters_at & H£)".
-        iMod (waiters_delete with "Hwaiters_auth Hwaiters_at") as "(%Hwaiters_lookup & Hwaiters_auth)".
-        iDestruct (big_sepM_delete with "Hwaiters") as "((%Ψ_ & Hwaiter_ & HΨ) & Hwaiters)"; first done.
-        iDestruct (saved_pred_agree true with "Hwaiter Hwaiter_") as "Heq".
-        iMod (lc_fupd_elim_later with "H£ Heq") as "Heq".
-        rewrite decide_False; first lia.
-
-        iMod "HΨ" as "(%vs & Hmodel₁ & _ & HΨ)".
-        iDestruct (model_agree with "Hmodel₁ Hmodel₂") as %->.
-        iMod ("HΨ" with "Hmodel₁") as "HΨ".
-
-        iSplitR "Heq HΨ HΦ". { iFrameSteps. }
-        iIntros "!> {%}".
-
-        iApply "HΦ".
-        iLeft. iRewrite "Heq". iSteps.
-
-      + iMod "Hop" as "(%vs & Hmodel₁ & _ & HΨ)".
-        iDestruct (model_agree with "Hmodel₁ Hmodel₂") as %->.
-        iMod ("HΨ" with "Hmodel₁") as "HΨ".
-
-        iSplitR "HΨ HΦ". { iFrameSteps. }
-        iSteps.
-  Qed.
-  #[local] Lemma next_spec {l γ i} node :
-    {{{
-      inv' l γ ∗
-      history_at γ i node
-    }}}
-      (#node).{next}
-    {{{ res,
-      RET res;
-        ⌜res = §Null%V⌝
-      ∨ ∃ node',
-        ⌜res = #node'⌝ ∗
-        node_model γ node' (S i) false
-    }}}.
-  Proof.
-    iIntros "%Φ (#Hinv & #Hhistory_at_node) HΦ".
-    wp_apply (next_spec_aux Other); iSteps.
-  Qed.
-  #[local] Lemma next_spec_is_empty {l γ i node} waiter Ψ :
-    {{{
-      inv' l γ ∗
-      history_at γ i node ∗
-      front_lb γ i ∗
-      saved_pred waiter Ψ ∗
-      waiters_at γ waiter i ∗
-      £ 1
-    }}}
-      (#node).{next}
-    {{{ res,
-      RET res;
-        ⌜res = §Null%V⌝ ∗
-        Ψ true
-      ∨ ∃ node',
-        ⌜res = #node'⌝ ∗
-        node_model γ node' (S i) false ∗
-        Ψ false
-    }}}.
-  Proof.
-    iIntros "%Φ (#Hinv & #Hhistory_at_node & #Hfront_lb_node & #Hwaiter & Hwaiters_at & H£) HΦ".
-    wp_apply (next_spec_aux (IsEmpty _ _) with "[$]").
-    iSteps.
-  Qed.
-  #[local] Lemma next_spec_pop {l γ i node} Ψ :
-    {{{
-      inv' l γ ∗
-      history_at γ i node ∗
-      front_lb γ i ∗
-      pop_au γ Ψ
-    }}}
-      (#node).{next}
-    {{{ res,
-      RET res;
-        ⌜res = §Null%V⌝ ∗
-        Ψ None
-      ∨ ∃ node',
-        ⌜res = #node'⌝ ∗
-        node_model γ node' (S i) false ∗
-        pop_au γ Ψ
-    }}}.
-  Proof.
-    iIntros "%Φ (#Hinv & #Hhistory_at_node & #Hfront_lb_node & Hau) HΦ".
-    wp_apply (next_spec_aux (Pop _) with "[$]").
+    iApply wp_fupd.
+    wp_apply (base.mpmc_queue_1_create_spec with "[//]") as (𝑡 γ) "(Hmeta & Hinv & Hmodel)".
+    iMod (meta_set γ with "Hmeta"); first done.
     iSteps.
   Qed.
 
@@ -690,19 +998,11 @@ Section mpmc_queue_1_G.
   Proof.
     iIntros "%Φ (:inv) HΦ".
 
-    wp_rec credits:"H£".
-    iDestruct (lc_weaken 2 with "H£") as "(H£1 & H£2)"; first done.
-    iDestruct (atomic_update_frame_l with "[H£1 $HΦ]") as "HΦ"; first iAccu.
-
-    wp_smart_apply (front_spec_strong (Some $ λ b, Φ #b) with "[$Hinv HΦ]")
-    as (node i) "((:node_model =node front=) & %waiter & #Hwaiter & Hwaiters_at)".
-    { rewrite /= /waiter_au. iAuIntro.
-      iApply (aacc_aupd_commit with "HΦ"); first done. iIntros "%vs (:model)". injection Heq as <-.
-      iDestruct (meta_agree with "Hmeta Hmeta_") as %<-. iClear "Hmeta_".
-      iAaccIntro with "Hmodel₁"; iSteps.
+    awp_apply (base.mpmc_queue_1_is_empty_spec with "[$]").
+    { iApply (aacc_aupd_commit with "HΦ"); first done. iIntros "%vs (:model =1)". simplify.
+      iDestruct (meta_agree with "Hmeta Hmeta_1") as %<-. iClear "Hmeta_1".
+      iAaccIntro with "Hmodel_1"; iSteps.
     }
-    wp_match.
-    wp_smart_apply (next_spec_is_empty with "[$]"); iSteps.
   Qed.
   Lemma mpmc_queue_1_is_empty_spec' t ι :
     {{{
@@ -716,109 +1016,7 @@ Section mpmc_queue_1_G.
   Proof.
     iIntros "%Φ (:inv) HΦ".
 
-    wp_rec.
-    wp_apply (front_spec with "Hinv") as (front i) "(:node_model =front front=)".
-    wp_match.
-    wp_apply (next_spec with "[$]") as (res) "[-> | (%node & -> & _)]"; iSteps.
-  Qed.
-
-  #[local] Lemma mpmc_queue_1_push_0_spec l γ i node new_back v :
-    <<<
-      meta l nroot γ ∗
-      inv' l γ ∗
-      node_model γ node i false ∗
-      new_back ↦ₕ Header §Node 2 ∗
-      new_back.[next] ↦ §Null ∗
-      new_back.[data] ↦ v
-    | ∀∀ vs,
-      mpmc_queue_1_model #l vs
-    >>>
-      mpmc_queue_1_push_0 #node #new_back @ ↑γ.(metadata_inv)
-    <<<
-      mpmc_queue_1_model #l (vs ++ [v])
-    | RET ();
-      ∃ j,
-      history_at γ j new_back
-    >>>.
-  Proof.
-    iIntros "%Φ (#Hmeta & #Hinv & (:node_model =node) & #Hnew_back_header & Hnew_back_next & Hnew_back_data) HΦ".
-
-    iLöb as "HLöb" forall (i node) "Hnode_header Hhistory_at_node".
-
-    wp_rec. wp_match.
-    wp_smart_apply (next_spec with "[$]") as (res) "[-> | (%node' & -> & (:node_model =node'))]"; last iSteps.
-    wp_pures.
-
-    wp_bind (CAS _ _ _).
-    iInv "Hinv" as "(:inv_inner)".
-    iDestruct (history_at_lookup with "Hhistory_auth Hhistory_at_node") as %Hlookup.
-    iDestruct (xtchain_lookup with "Hhist") as "(Hhist1 & _ & Hnode & Hhist2)"; first done.
-    destruct (hist !! S i) as [node' |] eqn:Hlookup'; simpl.
-
-    - wp_cas as _ | [=].
-      iDestruct (xtchain_lookup_2 with "Hhist1 Hnode_header Hnode Hhist2") as "Hhist"; [done | rewrite Hlookup' // |].
-      iSplitR "Hnew_back_next Hnew_back_data HΦ". { iFrameSteps. }
-      iSteps.
-
-    - wp_cas as ? | _; first done.
-      iDestruct (xtchain_lookup_2 with "Hhist1 Hnode_header Hnode []") as "Hhist"; [done | rewrite Hlookup' // | ..].
-      { rewrite -(length_lookup_last hist i) // drop_all.
-        iApply xtchain_nil.
-      }
-      iDestruct (big_sepL2_snoc_2 with "Hnodes Hnew_back_data") as "Hnodes".
-      iDestruct (xtchain_snoc_2 with "Hhist Hnew_back_header Hnew_back_next") as "Hhist".
-      iMod (history_update new_back with "Hhistory_auth") as "(Hhistory_auth & #Hhistory_at_new_back)".
-
-      iMod "HΦ" as "(%vs_ & (:model) & _ & HΦ)". injection Heq as <-.
-      iDestruct (meta_agree with "Hmeta Hmeta_") as %<-. iClear "Hmeta_".
-      iDestruct (model_agree with "Hmodel₁ Hmodel₂") as %->.
-      iMod (model_update (vs ++ [v]) with "Hmodel₁ Hmodel₂") as "(Hmodel₁ & Hmodel₂)".
-      iMod ("HΦ" with "[Hmodel₁]") as "HΦ"; [iSteps.. |].
-
-      iSplitR "HΦ".
-      { iExists (hist ++ [new_back]), past, front, (nodes ++ [new_back]), back, (vs ++ [v]).
-        iSteps; iPureIntro.
-        - rewrite Hhist -assoc //.
-        - set_solver.
-      }
-      iSteps.
-  Qed.
-
-  #[local] Lemma mpmc_queue_1_fix_back_spec l γ i back j new_back :
-    {{{
-      meta l nroot γ ∗
-      inv' l γ ∗
-      history_at γ i back ∗
-      node_model γ new_back j false
-    }}}
-      mpmc_queue_1_fix_back #l #back #new_back
-    {{{
-      RET ();
-      True
-    }}}.
-  Proof.
-    iIntros "%Φ (#Hmeta & #Hinv & #Hhistory_at_back & (:node_model =new_back)) HΦ".
-
-    iLöb as "HLöb" forall (i back) "Hhistory_at_back".
-
-    wp_rec. wp_match.
-
-    wp_bind (_ and _)%E.
-    wp_apply (wp_wand itype_bool) as (res) "(%b & ->)".
-    { wp_smart_apply (next_spec new_back with "[$]") as (res) "[-> | (%new_back' & -> & (:node_model =new_back'))]"; last iSteps.
-      wp_pures.
-
-      wp_bind (CAS _ _ _).
-      iInv "Hinv" as "(:inv_inner =1)".
-      wp_cas as _ | [= ->]; first iSteps.
-      iDestruct (history_at_lookup with "Hhistory_auth Hhistory_at_new_back") as %Hnew_back%list_elem_of_lookup_2.
-      iSteps.
-    }
-
-    destruct b; last iSteps.
-    wp_smart_apply domain_yield_spec.
-    wp_smart_apply (back_spec with "Hinv") as (back' i') "(:node_model =back')".
-    iApply ("HLöb" with "HΦ Hhistory_at_back'").
+    wp_apply (base.mpmc_queue_1_is_empty_spec' with "[$] HΦ").
   Qed.
 
   Lemma mpmc_queue_1_push_spec t ι v :
@@ -836,87 +1034,13 @@ Section mpmc_queue_1_G.
   Proof.
     iIntros "%Φ (:inv) HΦ".
 
-    wp_rec credit:"H£".
-    iDestruct (atomic_update_frame_l with "[H£ $HΦ]") as "HΦ"; first iAccu.
-    wp_block new_back as "#Hnew_back_header" "_" "(Hnew_back_next & Hnew_back_data & _)".
-    wp_match.
-    wp_smart_apply (back_spec with "Hinv") as (back i) "(:node_model =back)".
-    wp_smart_apply (mpmc_queue_1_push_0_spec with "[$]").
-    iApply (atomic_update_wand with "HΦ"). iIntros "%vs HΦ (%j & #Hhistory_at_new_back)".
-    wp_smart_apply (mpmc_queue_1_fix_back_spec with "[]"); first iSteps.
-    iSteps.
+    awp_apply (base.mpmc_queue_1_push_spec with "[$]").
+    { iApply (aacc_aupd_commit with "HΦ"); first done. iIntros "%vs (:model =1)". simplify.
+      iDestruct (meta_agree with "Hmeta Hmeta_1") as %<-. iClear "Hmeta_1".
+      iAaccIntro with "Hmodel_1"; iSteps.
+    }
   Qed.
 
-  #[local] Lemma mpmc_queue_1_pop_spec_aux l γ :
-    <<<
-      inv' l γ
-    | ∀∀ vs,
-      model₁ γ vs
-    >>>
-      mpmc_queue_1_pop #l @ ↑γ.(metadata_inv)
-    <<<
-      model₁ γ (tail vs)
-    | RET head vs;
-      £ 1
-    >>>.
-  Proof.
-    iIntros "%Φ #Hinv HΦ".
-
-    iLöb as "HLöb".
-
-    wp_rec credit:"H£".
-    wp_smart_apply (front_spec with "Hinv") as (front i) "(:node_model =front front=)".
-    wp_match.
-    wp_smart_apply (next_spec_pop (λ o, _ -∗ Φ o)%I with "[$]") as (res) "[(-> & HΦ) | (%new_front & -> & (:node_model =new_front) & HΦ)]"; first iSteps.
-    wp_match. wp_pures.
-
-    wp_bind (CAS _ _ _).
-    iInv "Hinv" as "(:inv_inner =1)".
-    iDestruct (history_at_lookup with "Hhistory_auth Hhistory_at_new_front") as %Hlookup.
-    iDestruct (xtchain_lookup_acc with "Hhist") as "(_ & Hnode & Hhist)"; first done.
-    wp_cas as _ | [= <-]; first iSteps.
-    iDestruct ("Hhist" with "Hnode") as "Hhist".
-    iDestruct (history_at_lookup with "Hhistory_auth Hhistory_at_front") as %Hlookup_old.
-    iAssert ⌜length past1 = i⌝%I as %Hpast_length.
-    { iDestruct (xtchain_NoDup with "Hhist") as %Hnodup.
-      iPureIntro. eapply NoDup_lookup; try done.
-      rewrite Hhist1 list_lookup_middle //.
-    }
-    rewrite Hhist1 (assoc _ _ [_]) lookup_app_r length_app /= in Hlookup; first lia.
-    rewrite Nat.add_1_r Hpast_length Nat.sub_diag in Hlookup.
-    destruct nodes1 as [| node nodes1]; first done. injection Hlookup as ->.
-    rewrite (assoc _ _ [_]) in Hhist1.
-    iDestruct (big_sepL2_cons_inv_l with "Hnodes") as "(%v & %vs' & -> & Hfront_data & Hnodes)".
-    set past := past1 ++ [front].
-    iMod (front_update (length past) with "Hfront_auth") as "Hfront_auth".
-    { rewrite /past. simpl_length. lia. }
-    iDestruct (big_sepM_impl_thread_fupd _ (waiter_model γ past)%I with "Hwaiters Hmodel₂ [#]") as ">(Hwaiters & Hmodel₂)".
-    { iIntros "!> %waiter %j %Hlookup (%P & #Hwaiter & HP) Hmodel₂".
-      destruct (Nat.lt_trichotomy j (length past1)) as [Hj | [-> | Hj]].
-      - rewrite decide_True //.
-        rewrite /waiter_model. setoid_rewrite decide_True; last first.
-        { rewrite /past. simpl_length. lia. }
-        iSteps.
-      - rewrite decide_False; first lia.
-        rewrite /waiter_model. setoid_rewrite decide_True; last first.
-        { rewrite /past. simpl_length/=. lia. }
-        iMod "HP" as "(%vs & Hmodel₁ & _ & HP)".
-        iDestruct (model_agree with "Hmodel₁ Hmodel₂") as %->.
-        iSteps.
-      - rewrite decide_False; first lia.
-        rewrite /waiter_model. setoid_rewrite decide_False; last first.
-        { rewrite /past. simpl_length/=. lia. }
-        iSteps.
-    }
-
-    iMod "HΦ" as "(%vs & Hmodel₁ & _ & HΦ)".
-    iDestruct (model_agree with "Hmodel₁ Hmodel₂") as %->.
-    iMod (model_update vs' with "Hmodel₁ Hmodel₂") as "(Hmodel₁ & Hmodel₂)".
-    iMod ("HΦ" with "Hmodel₁") as "HΦ".
-
-    iSplitR "Hfront_data H£ HΦ". { iFrameSteps. }
-    iSteps.
-  Qed.
   Lemma mpmc_queue_1_pop_spec t ι :
     <<<
       mpmc_queue_1_inv t ι
@@ -932,16 +1056,13 @@ Section mpmc_queue_1_G.
   Proof.
     iIntros "%Φ (:inv) HΦ".
 
-    wp_apply (mpmc_queue_1_pop_spec_aux with "Hinv").
-    iAuIntro.
-    iApply (aacc_aupd_commit with "HΦ"); first done. iIntros "%vs (:model)". injection Heq as <-.
-    iDestruct (meta_agree with "Hmeta Hmeta_") as %<-.
-    iAaccIntro with "Hmodel₁"; iSteps.
+    awp_apply (base.mpmc_queue_1_pop_spec with "[$]").
+    { iApply (aacc_aupd_commit with "HΦ"); first done. iIntros "%vs (:model =1)". simplify.
+      iDestruct (meta_agree with "Hmeta Hmeta_1") as %<-. iClear "Hmeta_1".
+      iAaccIntro with "Hmodel_1"; iSteps.
+    }
   Qed.
 End mpmc_queue_1_G.
-
-From zoo_saturn Require
-  mpmc_queue_1__opaque.
 
 #[global] Opaque mpmc_queue_1_inv.
 #[global] Opaque mpmc_queue_1_model.
